common/Separation.v
@@ -901,6 +901,7 @@ Proof.
 Qed.
 
 Context `{external_calls_ops: !ExternalCallsOps mem}.
+Context `{symbols_inject'_instance: !SymbolsInject}.
 Context `{external_calls_prf: !ExternalCalls mem}.
 
 Lemma external_call_parallel_rule:
